theories/LogicalRelation/Transitivity.v
@@ -505,7 +505,7 @@ Lemma kripkeLRlrefl `{GenericTypingProperties} {Γ l A A' B B'}
   (hB : forall Δ a b (ρ : Δ ≤ Γ) (wfΔ : [|-Δ])
     (hab : [hA Δ ρ wfΔ | Δ ||- a ≅ b : _]),
     [Δ ||-<l> B[a .: ρ >> tRel] ≅ B'[b .: ρ >> tRel]])
-  {Δ a b} (ρ : Δ ≤ Γ) (wfΔ : [|-Δ]) (hab : [hA Δ ρ wfΔ | Δ ||- a ≅ b : _]) :
+  [Δ a b] (ρ : Δ ≤ Γ) (wfΔ : [|-Δ]) (hab : [hA Δ ρ wfΔ | Δ ||- a ≅ b : _]) :
   [Δ ||-<l> B[a .: ρ >> tRel] ≅ B[b .: ρ >> tRel]].
 Proof.
   etransitivity; [eauto|].
@@ -517,7 +517,7 @@ Lemma kripkeLRurefl `{GenericTypingProperties} {Γ l A A' B B'}
   (hB : forall Δ a b (ρ : Δ ≤ Γ) (wfΔ : [|-Δ])
     (hab : [hA Δ ρ wfΔ | Δ ||- a ≅ b : _]),
     [Δ ||-<l> B[a .: ρ >> tRel] ≅ B'[b .: ρ >> tRel]])
-  {Δ a b} (ρ : Δ ≤ Γ) (wfΔ : [|-Δ]) (hab : [hA Δ ρ wfΔ | Δ ||- a ≅ b : _]) :
+  [Δ a b] (ρ : Δ ≤ Γ) (wfΔ : [|-Δ]) (hab : [hA Δ ρ wfΔ | Δ ||- a ≅ b : _]) :
   [Δ ||-<l> B'[a .: ρ >> tRel] ≅ B'[b .: ρ >> tRel]].
 Proof.
   eapply kripkeLRlrefl; tea; intros; symmetry; eapply hB; now symmetry.
