theories/Validity/Introductions/Empty.v
@@ -1,38 +1,30 @@
 From Coq Require Import CRelationClasses.
 From LogRel Require Import Utils Syntax.All GenericTyping LogicalRelation.
-From LogRel.LogicalRelation Require Import  Induction  Escape Irrelevance Reflexivity Irrelevance Weakening Neutral Transitivity Reduction Application EqRedRight.
+From LogRel.LogicalRelation Require Import  Properties.
 From LogRel.LogicalRelation.Introductions Require Import Universe SimpleArr.
-From LogRel.Validity Require Import Validity Irrelevance Properties Conversion SingleSubst Reflexivity Reduction Universe Pi SimpleArr Var Application.
+From LogRel.Validity Require Import Validity Irrelevance Properties Universe Pi SimpleArr Var Application.
+From Equations Require Import Equations.
 
 Set Universe Polymorphism.
+Set Printing Primitive Projection Parameters.
 
 Section Empty.
 Context `{GenericTypingProperties}.
 
 Set Printing Primitive Projection Parameters.
 
+Lemma emptyRedTy {Γ} : [|- Γ] -> [Γ ||-Empty tEmpty ≅ tEmpty].
+Proof. intros; constructor; eapply redtywf_refl; gen_typing. Defined.
 
 Lemma emptyRed {Γ l} : [|- Γ] -> [Γ ||-<l> tEmpty].
+Proof. intros; now apply LREmpty_, emptyRedTy. Defined.
+
+Lemma emptyValid {Γ Γ' l} (VΓ : [||-v Γ ≅ Γ']) : [Γ ||-v<l> tEmpty | VΓ].
 Proof.
-  intros; eapply LREmpty_; constructor; eapply redtywf_refl; gen_typing.
+  constructor; intros; now apply emptyRed.
 Defined.
 
-Lemma emptyValid {Γ l} (VΓ : [||-v Γ]) : [Γ ||-v<l> tEmpty | VΓ].
-Proof.
-  unshelve econstructor; intros.
-  + now eapply emptyRed.
-  + cbn; constructor; eapply redtywf_refl; gen_typing.
-Defined.
-
-Lemma emptyconvValid {Γ l} (VΓ : [||-v Γ]) (VEmpty : [Γ ||-v<l> tEmpty | VΓ]) :
-  [Γ ||-v<l> tEmpty ≅ tEmpty | VΓ | VEmpty].
-Proof.
-  constructor; intros.
-  enough [Δ ||-<l> tEmpty ≅ tEmpty | emptyRed wfΔ] by irrelevance.
-  constructor; cbn; eapply redtywf_refl; gen_typing.
-Qed.
-
-Lemma emptyURedTm {Δ} (wfΔ : [|-Δ]) : URedTm (LogRelRec one) Δ tEmpty U (redUOneCtx wfΔ).
+Lemma emptyURedTm {Δ l} (wfΔ : [|-Δ]) : URedTm l Δ tEmpty.
 Proof.
   exists tEmpty; [| constructor].
   eapply redtmwf_refl; gen_typing.
@@ -40,99 +32,77 @@ Defined.
 
 Lemma emptyTermRed {Δ} (wfΔ : [|-Δ]) : [Δ ||-<one> tEmpty : U | LRU_ (redUOneCtx wfΔ)].
 Proof.
-  unshelve eexists (emptyURedTm wfΔ) (emptyURedTm wfΔ) _; cbn.
-  1,3: now eapply (emptyRed (l:=zero)).
-  1: gen_typing.
-  apply reflLRTyEq.
+  unshelve eexists (emptyURedTm wfΔ) (emptyURedTm wfΔ); cbn.
+  1: gtyping.
+  now eapply (emptyRed (l:=zero)).
 Defined.
 
-Lemma emptyTermValid {Γ} (VΓ : [||-v Γ]):  [Γ ||-v<one> tEmpty : U | VΓ | UValid VΓ].
+Lemma emptyTermValid {Γ Γ'} (VΓ : [||-v Γ ≅ Γ']):  [Γ ||-v<one> tEmpty : U | VΓ | UValid VΓ].
 Proof.
   constructor; intros; eapply emptyTermRed.
 Qed.
 
+
+(* TODO : move *)
 Lemma liftSubst_singleSubst_eq {t u v: term} : t[u]⇑[v..] = t[u[v..]..].
 Proof. now bsimpl. Qed.
-
-(* TODO: move in Neutral *)
-Lemma NeNfRed {Γ l A n n'} (RA : [Γ ||-<l> A]) : [Γ ||-NeNf n ≅ n' : A] -> [RA | Γ ||- n ≅ n' : A].
-Proof.  intros []; now eapply neuTermEq. Qed.
 
 Section EmptyElimRedEq.
   Context {Γ l P Q}
     (wfΓ : [|- Γ])
-    (NN : [Γ ||-Empty tEmpty])
+    (NN : [Γ ||-Empty tEmpty ≅ tEmpty])
     (RN := LREmpty_ _ NN)
-    (RP : [Γ,, tEmpty ||-<l> P])
-    (RQ : [Γ,, tEmpty ||-<l> Q])
+    (WtP : [Γ,, tEmpty |- P])
+    (WtQ : [Γ,, tEmpty |- Q])
     (eqPQ : [Γ,, tEmpty |- P ≅ Q])
-    (RPpt : forall n n', [Γ ||-<l> n ≅ n' : _ | RN] -> [Γ ||-<l> P[n..]])
-    (RPQext : forall n n' (Rn : [Γ ||-<l> n ≅ n' : _ | RN]),
-      [Γ ||-<l> P[n..] ≅ Q[n'..] | RPpt _ _ Rn]).
-
-  #[local]
-  Lemma RQpt : forall n n', [Γ ||-<l> n ≅ n': _ | RN] -> [Γ ||-<l> Q[n..]].
-  Proof. intros; now unshelve eapply LRTyEqRedRight, RPQext. Qed.
+    (RPQext : forall n n', [Γ ||-<l> n ≅ n' : _ | RN] -> [Γ ||-<l> P[n..] ≅ Q[n'..]]).
 
   #[local]
   Lemma RPext : forall n n' (Rn : [Γ ||-<l> n ≅ n' : _ | RN]),
-      [Γ ||-<l> P[n..] ≅ P[n'..] | RPpt _ _ Rn].
+      [Γ ||-<l> P[n..] ≅ P[n'..] ].
   Proof.
-    intros; eapply transEq; [| eapply LRTyEqSym ].
-    all: unshelve (eapply RPQext; cycle 1; tea); now eapply urefl.
-    Unshelve. 2: eapply RQpt; now symmetry.
+    intros; etransitivity; [|symmetry];  eapply RPQext; tea; now eapply urefl.
   Qed.
 
   Lemma emptyElimRedEq n n' (Rnn' : [Γ ||-<l> n ≅ n' : _ | RN]) :
-    [Γ ||-<l> tEmptyElim P n ≅ tEmptyElim Q n' : _ | RPpt _ _ Rnn' ].
+    [Γ ||-<l> tEmptyElim P n ≅ tEmptyElim Q n' : _ | RPQext _ _ Rnn' ].
   Proof.
-    inversion Rnn'  as [??????? prop]; subst.
-    inversion prop as [?? h]; pose proof h as [?? conv]; subst.
-    pose proof (convneu_whne conv); pose proof (convneu_whne (symmetry conv)).
-    pose proof (Rne := neNfTermEq RN h); pose proof (Rnne := redwfSubstTmEq _ (lrefl Rne) redL).
-    pose proof (RPQext _ _ Rne).
-    escape.
-    eapply redSubstTmEq; cycle 1.
+    pose proof (redTmFwd' Rnn') as [].
+    depelim Rnn' ; eapply redSubstTmEq; cycle 1.
     + eapply redtm_emptyelim; tea; gen_typing.
     + eapply redtm_emptyelim; tea; gen_typing.
-    + now unshelve eapply escapeEq, RPQext.
-    + eapply LRTmEqConv; [unshelve eapply RPext;[|now symmetry]|].
-      eapply neuTermEq.
-      * eapply ty_emptyElim; tea.
-      * eapply ty_conv; [now eapply ty_emptyElim|now symmetry].
-      * now eapply convneu_emptyElim.
+    + destruct eq; eapply irrLRConv.
+      (* gtyping/gen_typing not working well here... *)
+      2: eapply neNfTermEq; constructor; [now eapply ty_emptyElim |..].
+      - eapply RPext; now symmetry.
+      - eapply ty_conv; [now eapply ty_emptyElim|].
+        symmetry; now eapply escapeEq, RPQext.
+      - now eapply convneu_emptyElim.
+      Unshelve. now eapply lrefl, RPQext.
   Qed.
 End EmptyElimRedEq.
 
 
 Section EmptyElimValid.
-  Context {Γ l}
-    (VΓ : [||-v Γ])
+  Context {Γ Γ' l}
+    (VΓ : [||-v Γ ≅ Γ'])
     (VN := emptyValid (l:=l) VΓ)
     (VΓN := validSnoc VΓ VN)
     { P P' }
-    (VP : [Γ ,, tEmpty ||-v<l> P | VΓN])
-    (VPP' : [Γ ,, tEmpty ||-v<l> P ≅ P' | VΓN | VP ])
-    (VP' := ureflValidTy VPP').
+    (VP : [Γ ,, tEmpty ||-v<l> P ≅ P' | VΓN]).
 
   Lemma emptyElimCongValid {n n'}
     (Vn : [Γ ||-v<l> n ≅ n' : tEmpty | VΓ | VN])
     (VPn := substS VP Vn)
     : [Γ ||-v<l> tEmptyElim P n ≅ tEmptyElim P' n' : _ | VΓ | VPn].
   Proof.
-    constructor; intros; instValid Vσσ'; epose proof (Vuσ := liftSubstEq' VN Vσσ').
+    constructor; intros; instValid Vσσ'; epose proof (Vuσ := liftSubst' VN Vσσ').
     instValid Vuσ; cbn in *; escape.
-    irrelevance0. 1: now rewrite singleSubstComm'.
-    eapply emptyElimRedEq; rewrite ?elimSuccHypTy_subst; tea.
-    + intros; irrelevance0; rewrite up_single_subst; [reflexivity|].
-      unshelve eapply validTyEq; cycle 1 ; tea.
-      now unshelve eapply consSubstEq.
-    Unshelve.
-      2: tea.
-      intros ?? Rn; rewrite up_single_subst.
-      unshelve eapply validTy.
-      5: tea.
-      3: unshelve eapply consSubstEq; tea.
+    eapply irrLREq. 1: now rewrite singleSubstComm'.
+    unshelve eapply emptyElimRedEq; rewrite ?elimSuccHypTy_subst; tea.
+    + now apply emptyRedTy.
+    + intros ; rewrite 2!up_single_subst; eapply validTyExt; tea.
+      now unshelve econstructor.
   Qed.
 End EmptyElimValid.
 
@@ -145,8 +115,7 @@ Lemma emptyElimValid {Γ l P n n'}
     (VPn := substS VP Vn):
     [Γ ||-v<l> tEmptyElim P n : _ | VΓ | VPn].
 Proof.
-  eapply lreflValidTm , emptyElimCongValid; tea.
-  now eapply reflValidTy.
+  eapply lrefl , emptyElimCongValid; tea.
 Qed.
 
 End Empty.
