theories/Validity/ValidityTactics.v
@@ -1,0 +1,200 @@
+From Ltac2 Require Import Ltac2 Printf.
+From Coq Require Import CRelationClasses.
+From LogRel Require Import Utils Syntax.All GenericTyping LogicalRelation.
+From LogRel.Validity Require Import Validity Irrelevance Properties PERTactics.
+
+
+Set Universe Polymorphism.
+Set Printing Primitive Projection Parameters.
+
+
+#[projections(primitive)]
+Record nprod {A B : Type} := pair { nfst : A ; nsnd : B }.
+Arguments nprod : clear implicits.
+Arguments pair {_ _} _ _.
+Notation "x <&> y" := (nprod x y) (at level 80, right associativity).
+
+#[projections(primitive)]
+Record sum {A : Type} {B : A -> Type} :=
+  dpair { dfst : A ; dsnd : B dfst }.
+Arguments sum : clear implicits.
+Arguments dpair {_ _} _ _.
+
+Notation "'∑&' x .. y , p" := (sum _ (fun x => .. (sum _ (fun y => p%type)) ..))
+  (at level 200, x binder, right associativity,
+   format "'[' '∑&'  '/  ' x  ..  y ,  '/  ' p ']'")
+  : type_scope.
+
+Definition packed_valid_ty `{GenericTypingProperties} l : crelation (context <&> term) :=
+  fun p1 p2 => ∑& (VΓ : [||-v nfst p1 ≅ nfst p2]), [_ ||-v<l> nsnd p1 ≅ nsnd p2 | VΓ].
+
+Instance packed_valid_tyPER `{GenericTypingProperties} l : PER (packed_valid_ty l).
+Proof.
+  constructor.
+  - intros ?? []; econstructor; now eapply symValidTy'.
+  - intros ??? [? xy] [? yz]; unshelve (econstructor; eapply transValidTy> [exact xy | exact yz]).
+    now etransitivity.
+Qed.
+
+Definition mkVty `{GenericTypingProperties} {l Γ Γ' A A'} {VΓ : [||-v Γ ≅ Γ']} (VA : [_ ||-v<l> A ≅ A' | VΓ]) :
+  packed_valid_ty l (pair Γ A) (pair Γ' A') :=
+  dpair VΓ VA.
+
+Definition packed_valid_tm `{GenericTypingProperties} l : crelation ((context <&> term) <&> term) :=
+  fun p1 p2 => ∑& (VΓA : packed_valid_ty l (nfst p1) (nfst p2)), [_ ||-v<l> nsnd p1 ≅ nsnd p2 : _ | dfst VΓA | dsnd VΓA].
+
+Instance packed_valid_tmPER `{GenericTypingProperties} l : PER (packed_valid_tm l).
+Proof.
+  constructor.
+  - intros ?? []; unshelve (econstructor;  now eapply symValidTm); now symmetry.
+  - intros ??? [? xy] [? yz].
+    unshelve (econstructor; eapply transValidTm > [exact xy | exact yz]).
+    now etransitivity.
+Qed.
+
+
+Definition mkVtm `{GenericTypingProperties} {l Γ Γ' A A' t t'} {VΓ : [||-v Γ ≅ Γ']} {VA : [_ ||-v<l> A ≅ A' | VΓ]} (Vt : [_ ||-v<l> t ≅ t' : _ | VΓ | VA]) :
+  packed_valid_tm l (pair (pair Γ A) t) (pair (pair Γ' A') t') :=
+  dpair (mkVty VA) Vt.
+
+Ltac2 mkvty c := constr:(mkVty $c).
+Ltac2 mkvtm c := constr:(mkVtm $c).
+Ltac2 pair a b := constr:(pair $a $b).
+
+Ltac2 valid_ctx_matcher ty pfopt :=
+  lazy_match! ty with
+  | VAdequate VR ?g ?g' => Some (g, g'), pfopt
+  | typeValidity ?g ?g' (VAd.pack ?vg) _ _ _ => Some (g, g'), Some vg
+  | termEqValidity ?g ?g' _ _ _ ?vg _ _ _ => Some (g, g'), Some vg
+  | _ => None, None
+  end.
+
+Ltac2 valid_ctx_rel h c :=
+  match valid_ctx_matcher c (Some (Control.hyp h)) with
+  | Some (g, g'), Some vg => [g,g',vg]
+  | _, _ => []
+  end.
+
+Ltac2 valid_ty_matcher ty pfopt :=
+  lazy_match! ty with
+  | typeValidity ?g ?g' (VAd.pack ?vg) ?l ?a ?a' => Some (g, g', vg, a, a', l), pfopt
+  | termEqValidity ?g ?g' ?l ?a ?a' ?vg ?va _ _ => Some (g, g', vg, a, a', l), Some va
+  | _ => None, None
+  end.
+
+Ltac2 valid_ty_rel st h c :=
+  match valid_ty_matcher c (Some (Control.hyp h)) with
+  | Some (g, _g', vg, a, a', _l), Some va =>
+    let (g0, wgg0) := Option.get_bt (PER.repr st g) in
+    let va0 := mkvty constr:(irrValidTy (VΓ0:=$vg) (VΓ1:=urefl $wgg0) $wgg0 $va) in
+    [pair g0 a, pair g0 a',  va0 ]
+  | _, _ => []
+  end.
+
+
+Ltac2 valid_tm_matcher ty pfopt :=
+  lazy_match! ty with
+  | termEqValidity ?g ?g' ?_l ?a ?a' ?_vg ?va ?t ?t' => Some (pair g a, pair g' a', mkvty va, t, t'), pfopt
+  | _ => None, None
+  end.
+
+Definition ureflValidTy `{GenericTypingProperties} {Γ Γ' l A B} {VΓ : [||-v Γ ≅ Γ']} (VΓ' := urefl VΓ) :
+  [Γ ||-v<l> A ≅ B | VΓ] -> [_ ||-v<l> B ≅ B | VΓ'].
+Proof. apply ureflValidTy. Defined.
+
+Ltac2 valid_tm_rel st h c :=
+  lazy_match! c with
+  | termEqValidity ?g ?_g' ?_l ?a ?_a' ?_vg ?va ?t ?t' =>
+    let h := Control.hyp h in
+    let (g0, wgg0) := Option.get_bt (PER.repr st g) in
+    (* let va0 := mkvty constr:(irrValidTy (VΓ0:=$vg) (VΓ1:=urefl $wgg0) $wgg0 $va) in *)
+    let (ga0, waa0) := Option.get_bt (PER.repr st (pair g0 a)) in
+    let vaa0 := constr:(convValidTy' _ $wgg0 (dsnd $waa0)) in
+    let vt0 := mkvtm constr:(irrValidTm $wgg0 $va (ureflValidTy $vaa0) $vaa0 $h) in
+    [pair ga0 t, pair ga0 t', vt0]
+  | _ => []
+  end.
+
+Ltac2 fail s := Control.throw (Tactic_failure (Some (Message.of_string s))).
+
+Ltac2 solve_ctx st g g' :=
+  match PER.get_witness_cstr st (g, g') with
+  | Some w => Control.refine (fun _ => w)
+  | None => fail "Contexts are not convertibles"
+  end.
+
+Ltac2 solve_ty st g _g' vg _l a a' :=
+  let (g0, wgg0) := Option.get_bt (PER.repr st g) in
+  match PER.get_witness_cstr st (pair g0 a, pair g0 a') with
+  | Some w => Control.refine (fun _ => constr:(irrValidTy (VΓ1:=$vg) (symmetry $wgg0) (dsnd $w)))
+  | None => fail "Types are not convertibles"
+  end.
+
+Ltac2 solve_tm st g _g' vg a _a' va _l t t' :=
+  let (g0, wgg0) := Option.get_bt (PER.repr st g) in
+  let (ga0, waa0) := Option.get_bt (PER.repr st (pair g0 a)) in
+  match PER.get_witness_cstr st (pair ga0 t, pair ga0 t') with
+  | Some w =>
+    let va0a := constr:(convValidTy _ (symmetry $wgg0) (dsnd (symmetry $waa0))) in
+    Control.refine (fun _ => constr:(irrValidTm (VΓ1:=$vg) (symmetry $wgg0) _ $va $va0a (dsnd $w)))
+  | None => fail "Terms are not convertibles"
+  end.
+
+Ltac2 solve_any st g :=
+  lazy_match! g with
+  | VAdequate VR ?g ?g' => solve_ctx st g g'
+  | typeValidity ?g ?g' (VAd.pack ?vg) ?l ?a ?a' => solve_ty st g g' vg l a a'
+  | termEqValidity ?g ?g' ?l ?a ?a' ?vg ?va ?t ?t' => solve_tm st g g' vg a a' va l t t'
+  | _ => fail "Term does not match"
+  end.
+
+Ltac2 init n :=
+  let st := PER.make n in
+  List.iter (PER.add_rel st valid_ctx_rel) (Control.hyps ()) ;
+  List.iter (PER.add_rel st (valid_ty_rel st)) (Control.hyps ()) ;
+  List.iter (PER.add_rel st (valid_tm_rel st)) (Control.hyps ()) ; st.
+
+Ltac2 irrValid () := let st := init 42 in solve_any st (Control.goal ()).
+
+Ltac irrValid := ltac2:(Control.enter irrValid).
+
+
+Module Examples.
+Section Examples.
+Context `{GenericTypingProperties}.
+
+Context {Γ0 Γ1 Γ2} (VΓ01 : [||-v Γ0 ≅ Γ1]) (VΓ02 : [||-v Γ0 ≅ Γ2]).
+
+Lemma VΓ12 : [||-v Γ1 ≅ Γ2].
+Proof.
+  irrValid ().
+Qed.
+
+Context {l A B C D} (VAB : [_ ||-v<l> A ≅ B | VΓ01]) (VDC : [_ ||-v<l> C ≅ D | VΓ12]).
+
+Lemma VBB2 (VΓ22 := urefl VΓ02) : [_ ||-v<l> B |VΓ22].
+Proof.
+  irrValid ().
+Qed.
+
+Lemma VAD10 (VΓ10 := symmetry VΓ01) (VCB : [_ ||-v<l> C ≅ B | VΓ12]) :
+  [_ ||-v<l> A ≅ D | VΓ10].
+Proof.
+  irrValid ().
+Qed.
+
+Context {t u v} (Vtu : [_ ||-v<l> t ≅ u : _ | _ | VAB]) (Vvu : [_ ||-v<l> v ≅ u : _ | _ | VBB2]).
+
+Lemma Vtt :  [_ ||-v<l> t ≅ t : _ | _ | VAB].
+Proof.
+  irrValid ().
+Qed.
+
+Lemma Vvt (VCB : [_ ||-v<l> C ≅ B | VΓ12]) : [_ ||-v<l> v ≅ t : _ | _ | VAD10 VCB].
+Proof.
+  irrValid ().
+Qed.
+
+End Examples.
+End Examples.
+
